Weidenbach_Book/Watched_Literals/Watched_Literals_List_Simp.thy
@@ -3,7 +3,17 @@ theory Watched_Literals_List_Simp
     Watched_Literals_List_Reduce
     Watched_Literals_List_Inprocessing
 begin
-
+lemma cdcl_twl_inprocessing_l_count_dec:
+  \<open>cdcl_twl_inprocessing_l S T \<Longrightarrow> count_decided (get_trail_l T) = count_decided (get_trail_l S)\<close>
+  by (induction rule: cdcl_twl_inprocessing_l.induct)
+   (auto simp: cdcl_twl_unitres_l.simps cdcl_twl_unitres_true_l.simps
+    cdcl_twl_subsumed_l.simps cdcl_twl_subresolution_l.simps)
+ 
+lemma rtranclp_cdcl_twl_inprocessing_l_count_dec:
+  \<open>cdcl_twl_inprocessing_l\<^sup>*\<^sup>* S T \<Longrightarrow> count_decided (get_trail_l T) = count_decided (get_trail_l S)\<close>
+  by (induction rule: rtranclp_induct)
+    (auto dest!: cdcl_twl_inprocessing_l_count_dec)
+    
 inductive cdcl_twl_restart_l_inp for S T where
   \<open>cdcl_twl_restart_l S T \<Longrightarrow> cdcl_twl_restart_l_inp S T\<close> |
   \<open>cdcl_twl_inprocessing_l S T \<Longrightarrow> cdcl_twl_restart_l_inp S T\<close>
@@ -31,6 +41,10 @@ lemma rtranclp_cdcl_twl_restart_l_inp_clauses_to_update_l:
       cdcl_twl_unitres_l.simps cdcl_twl_unitres_true_l.simps
       cdcl_twl_subsumed_l.simps cdcl_twl_subresolution_l.simps)
   done
+
+lemma rtranclp_cdcl_twl_inprocessing_l_cdcl_twl_l_inp:
+  \<open>cdcl_twl_inprocessing_l\<^sup>*\<^sup>* S T \<Longrightarrow> cdcl_twl_restart_l_inp\<^sup>*\<^sup>* S T\<close>
+  by (induction rule: rtranclp_induct) (auto dest!: cdcl_twl_restart_l_inp.intros)
 
 lemma cdcl_twl_restart_l_inp_cdcl_twl_restart_inp:
   assumes
@@ -93,20 +107,35 @@ definition cdcl_twl_full_restart_l_prog where
   RETURN T
   }\<close>
 
+definition cdcl_twl_full_restart_inprocess_l where
+  \<open>cdcl_twl_full_restart_inprocess_l S = do {
+  ASSERT(cdcl_twl_full_restart_l_GC_prog_pre S);
+  S' \<leftarrow> cdcl_twl_local_restart_l_spec0 S;
+  S' \<leftarrow> simplify_clauses_with_unit_st S';
+  if (get_conflict_l S' \<noteq> None) then
+    RETURN S'
+  else do {
+      T \<leftarrow> remove_one_annot_true_clause_imp S';
+      ASSERT(mark_to_delete_clauses_l_pre T);
+      U \<leftarrow> mark_to_delete_clauses_l T;
+      V \<leftarrow> cdcl_GC_clauses U;
+      ASSERT(cdcl_twl_restart_l_inp\<^sup>*\<^sup>* S V);
+      RETURN V
+    }
+  }\<close>
+
 definition cdcl_twl_full_restart_l_GC_prog where
   \<open>cdcl_twl_full_restart_l_GC_prog S = do {
     ASSERT(cdcl_twl_full_restart_l_GC_prog_pre S);
-  \<comment>\<open>\<^text>\<open>        S' \<leftarrow> cdcl_twl_local_restart_l_spec0 S;\<close>\<close>
-\<comment>\<open>\<^text>\<open>    S' \<leftarrow> simplify_clauses_with_unit_st S';\<close>\<close>
-    T \<leftarrow> remove_one_annot_true_clause_imp S;
+    S' \<leftarrow> cdcl_twl_local_restart_l_spec0 S;
+    T \<leftarrow> remove_one_annot_true_clause_imp S';
     ASSERT(mark_to_delete_clauses_l_pre T);
     U \<leftarrow> mark_to_delete_clauses_l T;
     V \<leftarrow> cdcl_GC_clauses U;
     ASSERT(cdcl_twl_restart_l S V);
     RETURN V
   }\<close>
-  (*
-  S' \<leftarrow> simplify_clauses_with_units_st S';*)
+
 
 context twl_restart_ops
 begin
@@ -228,14 +257,19 @@ where
          RETURN (T, size (get_all_learned_clss_l T), size (get_all_learned_clss_l T), n + 1)
        } else do {
          T \<leftarrow> SPEC(\<lambda>T. cdcl_twl_restart_l_inp\<^sup>*\<^sup>* S T \<and> count_decided (get_trail_l T) = 0);
-         T \<leftarrow> SPEC(\<lambda>U. cdcl_twl_restart_l T U);
-         T \<leftarrow> RETURN T;
-         RETURN (T, size (get_all_learned_clss_l T), size (get_all_learned_clss_l T), n + 1)
+         if get_conflict_l T = None
+         then do {
+           T \<leftarrow> SPEC(cdcl_twl_restart_l T);
+           T \<leftarrow> RETURN T;
+           RETURN (T, size (get_all_learned_clss_l T), size (get_all_learned_clss_l T), n + 1)
+         } else
+           RETURN (T, size (get_all_learned_clss_l T), size (get_all_learned_clss_l T), n + 1)
        }
      }
      else
        RETURN (S, last_GC, last_Restart, n)
    }\<close>
+
 
 lemma (in -)[twl_st_l]:
   \<open>(S, S') \<in> twl_st_l None \<Longrightarrow> get_learned_clss S' = twl_clause_of `# (get_learned_clss_l S)\<close>
@@ -474,8 +508,7 @@ lemma cdcl_twl_full_restart_l_GC_prog_cdcl_twl_restart_l:
     confl: \<open>get_conflict_l S = None\<close> and
     upd: \<open>clauses_to_update_l S = {#}\<close> and
     stgy_invs: \<open>twl_stgy_invs S'\<close> and
-    abs_pre: \<open>restart_prog_pre S' last_GC last_Restart brk\<close> and
-    lvl0: \<open>count_decided (get_trail_l S) = 0\<close>
+    abs_pre: \<open>restart_prog_pre S' last_GC last_Restart brk\<close>
   shows \<open>cdcl_twl_full_restart_l_GC_prog S \<le> \<Down> Id (SPEC (\<lambda>T. cdcl_twl_restart_l S T))\<close>
 proof -
   let ?f = \<open>(\<lambda>S T. cdcl_twl_restart_l S T)\<close>
@@ -490,7 +523,8 @@ proof -
       cdcl\<^sub>W_restart_mset.cdcl\<^sub>W_M_level_inv_def pcdcl_all_struct_invs_def
     by (simp add: twl_st)
   then have alt_def: \<open>SPEC (\<lambda>T. cdcl_twl_restart_l S T) \<ge> do {
-    T \<leftarrow> SPEC (?f2 S);
+    S' \<leftarrow> SPEC (\<lambda>S'. ?f1 S S');
+    T \<leftarrow> SPEC (?f2 S');
     U \<leftarrow> SPEC (?f3 T);
     V \<leftarrow> SPEC (\<lambda>V. ?f3 U V);
     RETURN V
@@ -502,26 +536,52 @@ proof -
     unfolding mem_Collect_eq
     by (metis (full_types) cdcl_twl_restart_l_cdcl_twl_restart_l_is_cdcl_twl_restart_l singletonD)
 
-  have 1: \<open>remove_one_annot_true_clause_imp S \<le> SPEC (\<lambda>V. ?f2 S V)\<close>
-    by (rule remove_one_annot_true_clause_imp_spec_lev0[OF assms(1-5) lvl0, THEN order_trans])
-     (use lvl0 remove_one_annot_true_clause_cdcl_twl_restart_l_spec[OF assms(1-4)] n_d
-	   remove_one_annot_true_clause_map_mark_of_same_or_0[of T] in
+  have 1: \<open>remove_one_annot_true_clause_imp T \<le> SPEC (\<lambda>V. ?f2 U V)\<close>
+    if
+      \<open>(T, U) \<in> Id\<close> and
+      \<open>U \<in> Collect (\<lambda>S'. ?f1 S S')\<close>
+    for T U
+  proof -
+    have \<open>T = U\<close> and \<open>?f S T \<or> S = T\<close> and count_0: \<open>count_decided (get_trail_l T) = 0\<close>
+      using that by auto
+    have confl: \<open>get_conflict_l T = None\<close>
+      using \<open>?f S T \<or> S = T\<close> confl
+      by (auto simp: cdcl_twl_restart_l.simps)
+    obtain T' where
+      TT': \<open>(T, T') \<in> twl_st_l None\<close> and
+      list_invs: \<open>twl_list_invs T\<close> and
+      struct_invs: \<open>twl_struct_invs T'\<close> and
+      clss_upd: \<open>clauses_to_update_l T = {#}\<close> and
+      \<open>cdcl_twl_restart S' T' \<or> S' = T'\<close>
+      using cdcl_twl_restart_l_invs[OF assms(1-3), of T] assms
+        \<open>?f S T \<or> S = T\<close>
+      by blast
+   show ?thesis
+      unfolding \<open>T = U\<close>[symmetric]
+      by (rule remove_one_annot_true_clause_imp_spec_lev0[OF TT' list_invs struct_invs confl
+          clss_upd, THEN order_trans])
+       (use count_0 remove_one_annot_true_clause_cdcl_twl_restart_l_spec[OF TT' list_invs struct_invs
+           confl clss_upd] n_d \<open>?f S T \<or> S = T\<close>
+           remove_one_annot_true_clause_map_mark_of_same_or_0[of T] in
          \<open>auto dest: cdcl_twl_restart_l_cdcl_twl_restart_l_is_cdcl_twl_restart_l
-	   simp: rtranclp_remove_one_annot_true_clause_count_dec\<close>)
+           simp: rtranclp_remove_one_annot_true_clause_count_dec\<close>)
+  qed
 
   have mark_to_delete_clauses_l_pre: \<open>mark_to_delete_clauses_l_pre U\<close>
     if
+      \<open>(T, T') \<in> Id\<close> and
+      \<open>T' \<in> Collect (?f1 S)\<close> and
       \<open>(U, U') \<in> Id\<close> and
-      \<open>U' \<in> Collect (?f2 S)\<close>
-    for U U'
+      \<open>U' \<in> Collect (?f2 T')\<close>
+    for T T' U U'
   proof -
-    have \<open>U = U'\<close> and \<open>?f S U\<close> 
+    have \<open>T = T'\<close> \<open>U = U'\<close> and \<open>?f T U\<close> and \<open>?f S T \<or> S = T\<close>
       using that by auto
     then have \<open>?f S U \<or> S = U\<close>
       using n_d cdcl_twl_restart_l_cdcl_twl_restart_l_is_cdcl_twl_restart_l
       by blast
     have confl: \<open>get_conflict_l U = None\<close>
-      using \<open>?f S U\<close> confl
+      using \<open>?f T U\<close> \<open>?f S T \<or> S = T\<close> confl
       by (auto simp: cdcl_twl_restart_l.simps)
     obtain U' where
       TT': \<open>(U, U') \<in> twl_st_l None\<close> and
@@ -537,17 +597,18 @@ proof -
   qed
   have 2: \<open>mark_to_delete_clauses_l U \<le> SPEC (\<lambda>V. ?f3 U' V)\<close>
     if
+      \<open>(T, T') \<in> Id\<close> and
+      \<open>T' \<in> Collect (?f1 S)\<close> and
       UU': \<open>(U, U') \<in> Id\<close> and
-      U: \<open>U' \<in> Collect (?f2 S)\<close> and
+      U: \<open>U' \<in> Collect (?f2 T')\<close> and
       pre: \<open>mark_to_delete_clauses_l_pre U\<close>
-    for U U'
+    for T T' U U'
   proof -
-    have \<open>U = U'\<close> and \<open>?f S U\<close>
+    have \<open>T = T'\<close> \<open>U = U'\<close> and \<open>?f T U\<close> and \<open>?f S T \<or> S = T\<close>
       using that by auto
     then have SU: \<open>?f S U\<close>
       using n_d cdcl_twl_restart_l_cdcl_twl_restart_l_is_cdcl_twl_restart_l
       by blast
-
     obtain V where
       TV: \<open>(U, V) \<in> twl_st_l None\<close> and
       struct: \<open>twl_struct_invs V\<close> and
@@ -555,27 +616,29 @@ proof -
       using pre unfolding mark_to_delete_clauses_l_pre_def
       by auto
     have confl: \<open>get_conflict_l U = None\<close> and upd: \<open>clauses_to_update_l U = {#}\<close> and UU[simp]: \<open>U' = U\<close>
-      using U UU' \<open>?f S U\<close> confl assms
+      using U UU' \<open>?f T U\<close> confl  \<open>?f S T \<or> S = T\<close> assms
       by (auto simp: cdcl_twl_restart_l.simps)
     show ?thesis
       by (rule mark_to_delete_clauses_l_spec[OF TV list_invs struct confl upd, THEN order_trans],
          subst Down_id_eq)
        (use remove_one_annot_true_clause_cdcl_twl_restart_l_spec[OF TV list_invs struct confl upd]
-          cdcl_twl_restart_l_cdcl_twl_restart_l_is_cdcl_twl_restart_l[OF _ _ n_d, of S] that lvl0
+          cdcl_twl_restart_l_cdcl_twl_restart_l_is_cdcl_twl_restart_l[OF _ _ n_d, of T] that
           ST in \<open>auto dest!: cdcl_twl_restart_l_count_dec\<close>)
   qed
   have 3: \<open>cdcl_GC_clauses V \<le> SPEC (?f3 V')\<close>
     if
+      \<open>(T, T') \<in> Id\<close> and
+      \<open>T' \<in> Collect (?f1 S)\<close> and
       \<open>(U, U') \<in> Id\<close> and
-      \<open>U' \<in> Collect (?f2 S)\<close> and
+      \<open>U' \<in> Collect (?f2 T')\<close> and
       \<open>mark_to_delete_clauses_l_pre U\<close> and
       \<open>(V, V') \<in> Id\<close> and
       \<open>V' \<in> Collect (?f3 U')\<close>
-    for  U U' V V'
+    for T T' U U' V V'
   proof -
     have eq: \<open>U' = U\<close>
       using that by auto
-    have st: \<open>U = U'\<close> \<open>V = V'\<close> and \<open>?f S U\<close> and
+    have st: \<open>T = T'\<close> \<open>U = U'\<close> \<open>V = V'\<close> and \<open>?f S T \<or> S = T\<close> and \<open>?f T U\<close> and
        \<open>?f U V \<or> U = V\<close> and
       le_UV: \<open>length (get_trail_l U) = length (get_trail_l V)\<close> and
       mark0: \<open>\<forall>L\<in>set (get_trail_l V'). mark_of L = 0\<close> and
@@ -610,15 +673,17 @@ proof -
   qed
   have cdcl_twl_restart_l: \<open>cdcl_twl_restart_l S W\<close>
     if
+      \<open>(T, T') \<in> Id\<close> and
+      \<open>T' \<in> Collect (?f1 S)\<close> and
       \<open>(U, U') \<in> Id\<close> and
-      \<open>U' \<in> Collect (?f2 S)\<close> and
+      \<open>U' \<in> Collect (?f2 T')\<close> and
       \<open>mark_to_delete_clauses_l_pre U\<close> and
       \<open>(V, V') \<in> Id\<close> and
       \<open>V' \<in> Collect (?f3 U')\<close> and
       \<open>(W, W') \<in> Id\<close> and
       \<open>W' \<in> Collect (?f3 V')\<close>
-    for U U' V V' W W'
-    using n_d
+    for T T' U U' V V' W W'
+    using n_d cdcl_twl_restart_l_cdcl_twl_restart_l_is_cdcl_twl_restart_l[of S T U]
       cdcl_twl_restart_l_cdcl_twl_restart_l_is_cdcl_twl_restart_l[of S U V]
       cdcl_twl_restart_l_cdcl_twl_restart_l_is_cdcl_twl_restart_l[of S V W] that
     by fast
@@ -638,8 +703,434 @@ proof -
       using assms unfolding cdcl_twl_full_restart_l_GC_prog_pre_def restart_prog_pre_def
       by fastforce
     subgoal
+      by (rule cdcl_twl_local_restart_l_spec0_cdcl_twl_restart_l[THEN order_trans, OF abs_pre])
+        auto
+    subgoal
       by (rule 1)
-    subgoal for U U'
+    subgoal for  T T' U U'
+      by (rule mark_to_delete_clauses_l_pre)
+    subgoal for T T' U U'
+      by (rule 2)
+    subgoal for T T' U U' V V'
+      by (rule 3)
+    subgoal for T T' U U' V V' W W'
+      by (rule cdcl_twl_restart_l)
+    done
+qed
+
+
+lemma cdcl_twl_full_restart_inprocess_l_cdcl_twl_restart_l:
+  assumes
+    ST: \<open>(S, S') \<in> twl_st_l None\<close> and
+    list_invs: \<open>twl_list_invs S\<close> and
+    struct_invs: \<open>twl_struct_invs S'\<close> and
+    confl: \<open>get_conflict_l S = None\<close> and
+    upd: \<open>clauses_to_update_l S = {#}\<close> and
+    stgy_invs: \<open>twl_stgy_invs S'\<close> and
+    abs_pre: \<open>restart_prog_pre S' last_GC last_Restart brk\<close>
+  shows \<open>cdcl_twl_full_restart_inprocess_l S \<le> \<Down> Id (SPEC (\<lambda>T. cdcl_twl_restart_l_inp\<^sup>*\<^sup>* S T \<and> count_decided (get_trail_l T) = 0))\<close> (is \<open>_ \<le> \<Down> _ ?P\<close>)
+proof -
+  let ?f = \<open>(\<lambda>S T. cdcl_twl_restart_l S T)\<close>
+  let ?f1 = \<open>\<lambda>S S'. (?f S S' \<or> S = S') \<and> count_decided (get_trail_l S') = 0\<close>
+  let ?f1' = \<open>\<lambda>S S'. (?f S S') \<and> count_decided (get_trail_l S') = 0\<close>
+  let ?finp = \<open>\<lambda>S S'. cdcl_twl_restart_l_inp\<^sup>*\<^sup>* S S' \<and>  count_decided (get_trail_l S') = 0\<close>
+  let ?f2 = \<open>\<lambda>S S'. ?f S S' \<and> (\<forall>L \<in> set (get_trail_l S'). mark_of L = 0) \<and>
+    length (get_trail_l S) = length (get_trail_l S')\<close>
+  let ?f3 = \<open>\<lambda>S S'. ?f1 S S' \<and> (\<forall>L \<in> set (get_trail_l S'). mark_of L = 0) \<and>
+    length (get_trail_l S) = length (get_trail_l S')\<close>
+  have n_d: \<open>no_dup (get_trail_l S)\<close>
+    using struct_invs ST unfolding twl_struct_invs_def cdcl\<^sub>W_restart_mset.cdcl\<^sub>W_all_struct_inv_def
+      cdcl\<^sub>W_restart_mset.cdcl\<^sub>W_M_level_inv_def pcdcl_all_struct_invs_def
+    by (simp add: twl_st)
+  then have alt_def: \<open>?P \<ge> do {
+    S' \<leftarrow> SPEC (?f1 S);
+    T \<leftarrow> SPEC (?finp S');
+    if(get_conflict_l T \<noteq> None) then
+      RETURN T
+    else do {
+        T \<leftarrow> SPEC (?f2 T);
+        U \<leftarrow> SPEC (?f3 T);
+        V \<leftarrow> SPEC (\<lambda>V. ?f3 U V);
+        RETURN V
+      }
+    }\<close>
+    unfolding RETURN_def RES_RES_RETURN_RES apply -
+    apply refine_vcg
+    apply (metis (no_types, hide_lams) cdcl_twl_restart_l_inp.intros(1) converse_rtranclp_into_rtranclp empty_iff insert_iff)
+    apply simp
+      apply (elim UN_E)+
+      unfolding mem_Collect_eq
+      apply (smt (z3) cdcl_twl_restart_l_inp.intros(1) converse_rtranclp_into_rtranclp rtranclp.rtrancl_into_rtrancl singletonD)
+      apply (elim UN_E)+
+      unfolding mem_Collect_eq
+      apply (metis (no_types, hide_lams) singletonD)
+    done
+
+  have 1: \<open>remove_one_annot_true_clause_imp U \<le> SPEC (?f2 U')\<close>
+    if 
+      \<open>cdcl_twl_full_restart_l_GC_prog_pre S\<close> and
+      \<open>T' \<in> Collect (?f1 S)\<close>  and
+      \<open>U' \<in> Collect (?finp T')\<close> and
+      confl_U': \<open>\<not>get_conflict_l U' \<noteq> None\<close> and
+      \<open>(T, T') \<in> Id\<close> and
+      \<open>(U, U') \<in> Id\<close>
+      for T T' U U'
+  proof -
+    have \<open>T = T'\<close> \<open>U=U'\<close> and \<open>?f S T \<or> S = T\<close> and
+      count_0: \<open>count_decided (get_trail_l T) = 0\<close> and
+      T'U': \<open>cdcl_twl_restart_l_inp\<^sup>*\<^sup>* T' U'\<close> and
+      count_0_U: \<open>count_decided (get_trail_l U') = 0\<close> and
+      confl_U': \<open>get_conflict_l U' = None\<close>
+      using that by auto
+    have confl: \<open>get_conflict_l T = None\<close>
+      using \<open>?f S T \<or> S = T\<close> confl
+      by (auto simp: cdcl_twl_restart_l.simps)
+    obtain T'' where
+      TT': \<open>(T', T'') \<in> twl_st_l None\<close> and
+      list_invs: \<open>twl_list_invs T'\<close> and
+      struct_invs: \<open>twl_struct_invs T''\<close> and
+      clss_upd: \<open>clauses_to_update_l T' = {#}\<close> and
+      \<open>cdcl_twl_restart S' T'' \<or> S' = T''\<close>
+      using cdcl_twl_restart_l_invs[OF assms(1-3), of T] assms
+        \<open>?f S T \<or> S = T\<close> unfolding  \<open>T = T'\<close>
+      by blast
+
+    have ent: \<open>cdcl\<^sub>W_restart_mset.cdcl\<^sub>W_learned_clauses_entailed_by_init (state\<^sub>W_of T'')\<close>
+      using \<open>cdcl_twl_restart S' T'' \<or> S' = T''\<close> abs_pre cdcl_twl_inp.intros(5)
+        cdcl_twl_inp_invs(3) restart_prog_pre_def by blast
+    obtain U'' where
+      U'U'': \<open>(U', U'') \<in> twl_st_l None\<close> and
+      \<open>cdcl_twl_inp\<^sup>*\<^sup>* T'' U''\<close>
+      using rtranclp_cdcl_twl_restart_l_inp_cdcl_twl_restart_inp[OF T'U' TT' list_invs struct_invs
+        ent] by blast
+    then have
+      list_invs: \<open>twl_list_invs U'\<close> and
+      struct_invs: \<open>twl_struct_invs U''\<close> and
+      clss_upd: \<open>clauses_to_update_l U' = {#}\<close>
+      using T'U' ent
+      by (auto intro:  list_invs rtranclp_cdcl_twl_restart_l_inp_twl_list_invs
+          rtranclp_cdcl_twl_inp_invs struct_invs
+        clss_upd rtranclp_cdcl_twl_restart_l_inp_clauses_to_update_l
+       simp: \<open>U = U'\<close>)
+
+   show ?thesis
+     unfolding \<open>T = T'\<close>[symmetric] \<open>U=U'\<close>
+      by (rule remove_one_annot_true_clause_imp_spec_lev0[OF U'U'' list_invs struct_invs confl_U'
+        clss_upd, THEN order_trans])
+       (use count_0 remove_one_annot_true_clause_cdcl_twl_restart_l_spec[OF U'U'' list_invs
+          struct_invs confl_U' clss_upd] n_d \<open>?f S T \<or> S = T\<close> count_0_U
+           remove_one_annot_true_clause_map_mark_of_same_or_0[of T] in
+         \<open>auto dest: cdcl_twl_restart_l_cdcl_twl_restart_l_is_cdcl_twl_restart_l
+           simp: rtranclp_remove_one_annot_true_clause_count_dec\<close>)
+  qed
+
+  have mark_to_delete_clauses_l_pre: \<open>mark_to_delete_clauses_l_pre V\<close>
+    if
+      \<open>T' \<in> Collect (?f1 S)\<close> and
+      \<open>U' \<in> Collect (?finp T')\<close> and
+      confl_U': \<open>\<not>get_conflict_l U' \<noteq> None\<close> and
+      \<open>V' \<in> Collect (?f2 U')\<close> and
+      \<open>(V, V') \<in> Id\<close> and
+      \<open>(T, T') \<in> Id\<close> and
+      \<open>(U, U') \<in> Id\<close>
+    for T T' U U' V V'
+  proof -
+    have \<open>T = T'\<close> \<open>U=U'\<close> \<open>V'=V\<close> and \<open>?f S T \<or> S = T\<close> and
+      count_0: \<open>count_decided (get_trail_l T) = 0\<close> and
+      T'U': \<open>cdcl_twl_restart_l_inp\<^sup>*\<^sup>* T' U'\<close> and
+      count_0_U: \<open>count_decided (get_trail_l U') = 0\<close> and
+      confl_U': \<open>get_conflict_l U' = None\<close> and
+      UV: \<open>cdcl_twl_restart_l U' V\<close>
+      using that by auto
+    have confl: \<open>get_conflict_l T = None\<close>
+      using \<open>?f S T \<or> S = T\<close> confl
+      by (auto simp: cdcl_twl_restart_l.simps)
+    obtain T'' where
+      TT': \<open>(T', T'') \<in> twl_st_l None\<close> and
+      list_invs: \<open>twl_list_invs T'\<close> and
+      struct_invs: \<open>twl_struct_invs T''\<close> and
+      clss_upd: \<open>clauses_to_update_l T' = {#}\<close> and
+      \<open>cdcl_twl_restart S' T'' \<or> S' = T''\<close>
+      using cdcl_twl_restart_l_invs[OF assms(1-3), of T] assms
+        \<open>?f S T \<or> S = T\<close> unfolding  \<open>T = T'\<close>
+      by blast
+
+    have ent: \<open>cdcl\<^sub>W_restart_mset.cdcl\<^sub>W_learned_clauses_entailed_by_init (state\<^sub>W_of T'')\<close>
+      using \<open>cdcl_twl_restart S' T'' \<or> S' = T''\<close> abs_pre cdcl_twl_inp.intros(5)
+        cdcl_twl_inp_invs(3) restart_prog_pre_def by blast
+    obtain U'' where
+      U'U'': \<open>(U', U'') \<in> twl_st_l None\<close> and
+      \<open>cdcl_twl_inp\<^sup>*\<^sup>* T'' U''\<close>
+      using rtranclp_cdcl_twl_restart_l_inp_cdcl_twl_restart_inp[OF T'U' TT' list_invs struct_invs
+        ent] by blast
+    then have
+      list_invs: \<open>twl_list_invs U'\<close> and
+      struct_invs: \<open>twl_struct_invs U''\<close> and
+      clss_upd: \<open>clauses_to_update_l U' = {#}\<close>
+      using T'U' ent
+      by (auto intro:  list_invs rtranclp_cdcl_twl_restart_l_inp_twl_list_invs
+          rtranclp_cdcl_twl_inp_invs struct_invs
+        clss_upd rtranclp_cdcl_twl_restart_l_inp_clauses_to_update_l
+       simp: \<open>U = U'\<close>)
+    obtain V'' where
+      \<open>(V, V'') \<in> twl_st_l None\<close>
+      \<open>twl_list_invs V\<close>
+      \<open>clauses_to_update_l V = {#}\<close>
+      \<open>cdcl_twl_restart U'' V''\<close>
+      \<open>twl_struct_invs V''\<close>
+      using cdcl_twl_restart_l_invs[OF U'U'' list_invs struct_invs UV]
+      by blast
+    then show ?thesis
+      unfolding mark_to_delete_clauses_l_pre_def  \<open>U=U'\<close>
+      by blast
+  qed
+
+  
+  have 2:  \<open>mark_to_delete_clauses_l V \<le> SPEC (?f3 V')\<close>
+    if
+      \<open>T' \<in> Collect (?f1 S)\<close> and
+      \<open>U' \<in> Collect (?finp T')\<close> and
+      confl_U': \<open>\<not>get_conflict_l U' \<noteq> None\<close> and
+      \<open>V' \<in> Collect (?f2 U')\<close> and
+      \<open>(V, V') \<in> Id\<close> and
+      \<open>(T, T') \<in> Id\<close> and
+      \<open>(U, U') \<in> Id\<close>
+    for T T' U U' V V'
+  proof -
+    have \<open>T = T'\<close> \<open>U=U'\<close> \<open>V'=V\<close> and \<open>?f S T \<or> S = T\<close> and
+      count_0: \<open>count_decided (get_trail_l T) = 0\<close> and
+      T'U': \<open>cdcl_twl_restart_l_inp\<^sup>*\<^sup>* T' U'\<close> and
+      count_0_U: \<open>count_decided (get_trail_l U') = 0\<close> and
+      confl_U': \<open>get_conflict_l U' = None\<close> and
+      UV: \<open>cdcl_twl_restart_l U' V\<close>
+      using that by auto
+    have confl: \<open>get_conflict_l T = None\<close>
+      using \<open>?f S T \<or> S = T\<close> confl
+      by (auto simp: cdcl_twl_restart_l.simps)
+    obtain T'' where
+      TT': \<open>(T', T'') \<in> twl_st_l None\<close> and
+      list_invs: \<open>twl_list_invs T'\<close> and
+      struct_invs: \<open>twl_struct_invs T''\<close> and
+      clss_upd: \<open>clauses_to_update_l T' = {#}\<close> and
+      \<open>cdcl_twl_restart S' T'' \<or> S' = T''\<close>
+      using cdcl_twl_restart_l_invs[OF assms(1-3), of T] assms
+        \<open>?f S T \<or> S = T\<close> unfolding  \<open>T = T'\<close>
+      by blast
+
+    have ent: \<open>cdcl\<^sub>W_restart_mset.cdcl\<^sub>W_learned_clauses_entailed_by_init (state\<^sub>W_of T'')\<close>
+      using \<open>cdcl_twl_restart S' T'' \<or> S' = T''\<close> abs_pre cdcl_twl_inp.intros(5)
+        cdcl_twl_inp_invs(3) restart_prog_pre_def by blast
+    obtain U'' where
+      U'U'': \<open>(U', U'') \<in> twl_st_l None\<close> and
+      \<open>cdcl_twl_inp\<^sup>*\<^sup>* T'' U''\<close>
+      using rtranclp_cdcl_twl_restart_l_inp_cdcl_twl_restart_inp[OF T'U' TT' list_invs struct_invs
+        ent] by blast
+    then have
+      list_invs: \<open>twl_list_invs U'\<close> and
+      struct_invs: \<open>twl_struct_invs U''\<close> and
+      clss_upd: \<open>clauses_to_update_l U' = {#}\<close>
+      using T'U' ent
+      by (auto intro:  list_invs rtranclp_cdcl_twl_restart_l_inp_twl_list_invs
+          rtranclp_cdcl_twl_inp_invs struct_invs
+        clss_upd rtranclp_cdcl_twl_restart_l_inp_clauses_to_update_l
+       simp: \<open>U = U'\<close>)
+    obtain V'' where
+      VV'': \<open>(V, V'') \<in> twl_st_l None\<close> and
+      list_invs: \<open>twl_list_invs V\<close> and
+      upd: \<open>clauses_to_update_l V = {#}\<close> and
+      U''V'': \<open>cdcl_twl_restart U'' V''\<close> and
+      struct_invs: \<open>twl_struct_invs V''\<close>
+      using cdcl_twl_restart_l_invs[OF U'U'' list_invs struct_invs UV]
+      by blast
+    have confl: \<open>get_conflict_l V = None\<close>
+      using U''V'' VV'' confl_U' U'U''
+      by (auto simp: cdcl_twl_restart.simps  \<open>U=U'\<close> \<open>V'=V\<close>
+          twl_st_l_def)
+    show ?thesis
+      by (rule mark_to_delete_clauses_l_spec[OF VV'' list_invs struct_invs confl upd,
+    THEN order_trans],
+        subst Down_id_eq)
+       (use confl remove_one_annot_true_clause_cdcl_twl_restart_l_spec[OF VV'' list_invs struct_invs _ upd]
+        cdcl_twl_restart_l_cdcl_twl_restart_l_is_cdcl_twl_restart_l[OF _ _ n_d, of T] that
+        ST in \<open>auto dest!: cdcl_twl_restart_l_count_dec\<close>)
+  qed
+
+  have 3: \<open>cdcl_GC_clauses W \<le> SPEC (?f3 W')\<close>
+    if
+      \<open>T' \<in> Collect (?f1 S)\<close> and
+      \<open>U' \<in> Collect (?finp T')\<close> and
+      confl_U': \<open>\<not>get_conflict_l U' \<noteq> None\<close> and
+      V': \<open>V' \<in> Collect (?f2 U')\<close> and
+      \<open>W' \<in> Collect (?f3 V')\<close> and
+      \<open>(V, V') \<in> Id\<close> and
+      \<open>(T, T') \<in> Id\<close> and
+      \<open>(U, U') \<in> Id\<close> and
+      \<open>(W, W') \<in> Id\<close>
+    for T T' U U' V V' W W'
+  proof -
+    have eq: \<open>T = T'\<close> \<open>U=U'\<close> \<open>V'=V\<close> \<open>W=W'\<close> and
+      \<open>?f S T \<or> S = T\<close> and
+      count_0: \<open>count_decided (get_trail_l T) = 0\<close> and
+      T'U': \<open>cdcl_twl_restart_l_inp\<^sup>*\<^sup>* T' U'\<close> and
+      count_0_U: \<open>count_decided (get_trail_l U') = 0\<close> and
+      confl_U': \<open>get_conflict_l U' = None\<close> and
+      UV: \<open>cdcl_twl_restart_l U' V\<close> and
+      VW: \<open>?f V W' \<or> V = W'\<close> and
+      mark: \<open>\<forall>L\<in>set (get_trail_l W'). mark_of L = 0\<close>
+      using that by auto
+    have confl: \<open>get_conflict_l T = None\<close>
+      using \<open>?f S T \<or> S = T\<close> confl
+      by (auto simp: cdcl_twl_restart_l.simps)
+    obtain T'' where
+      TT': \<open>(T', T'') \<in> twl_st_l None\<close> and
+      list_invs: \<open>twl_list_invs T'\<close> and
+      struct_invs: \<open>twl_struct_invs T''\<close> and
+      clss_upd: \<open>clauses_to_update_l T' = {#}\<close> and
+      \<open>cdcl_twl_restart S' T'' \<or> S' = T''\<close>
+      using cdcl_twl_restart_l_invs[OF assms(1-3), of T] assms
+        \<open>?f S T \<or> S = T\<close> unfolding  \<open>T = T'\<close>
+      by blast
+
+    have ent: \<open>cdcl\<^sub>W_restart_mset.cdcl\<^sub>W_learned_clauses_entailed_by_init (state\<^sub>W_of T'')\<close>
+      using \<open>cdcl_twl_restart S' T'' \<or> S' = T''\<close> abs_pre cdcl_twl_inp.intros(5)
+        cdcl_twl_inp_invs(3) restart_prog_pre_def by blast
+    obtain U'' where
+      U'U'': \<open>(U', U'') \<in> twl_st_l None\<close> and
+      \<open>cdcl_twl_inp\<^sup>*\<^sup>* T'' U''\<close>
+      using rtranclp_cdcl_twl_restart_l_inp_cdcl_twl_restart_inp[OF T'U' TT' list_invs struct_invs
+        ent] by blast
+    then have
+      list_invs: \<open>twl_list_invs U'\<close> and
+      struct_invs: \<open>twl_struct_invs U''\<close> and
+      clss_upd: \<open>clauses_to_update_l U' = {#}\<close>
+      using T'U' ent
+      by (auto intro:  list_invs rtranclp_cdcl_twl_restart_l_inp_twl_list_invs
+          rtranclp_cdcl_twl_inp_invs struct_invs
+        clss_upd rtranclp_cdcl_twl_restart_l_inp_clauses_to_update_l
+       simp: \<open>U = U'\<close>)
+    obtain V'' where
+      VV'': \<open>(V, V'') \<in> twl_st_l None\<close> and
+      list_invs: \<open>twl_list_invs V\<close> and
+      upd: \<open>clauses_to_update_l V = {#}\<close> and
+      U''V'': \<open>cdcl_twl_restart U'' V''\<close> and
+      struct_invs: \<open>twl_struct_invs V''\<close>
+      using cdcl_twl_restart_l_invs[OF U'U'' list_invs struct_invs UV]
+      by blast
+    have confl: \<open>get_conflict_l V = None\<close>
+      using U''V'' VV'' confl_U' U'U''
+     by (auto simp: cdcl_twl_restart.simps  \<open>U=U'\<close> \<open>V'=V\<close>
+          twl_st_l_def)
+    have count_0_V: \<open>count_decided (get_trail_l V) = 0\<close>
+      using count_0_U V' U'U'' unfolding eq
+      by (auto dest!: cdcl_twl_restart_l_count_dec)
+    obtain W'' where
+      VW'': \<open>(W, W'') \<in> twl_st_l None\<close> and
+      list_invs: \<open>twl_list_invs W\<close> and
+      upd: \<open>clauses_to_update_l W = {#}\<close> and
+      U''W'': \<open>cdcl_twl_restart V'' W'' \<or> V = W\<close> and
+      struct_invs: \<open>twl_struct_invs W''\<close>
+      using cdcl_twl_restart_l_invs[OF VV'' list_invs struct_invs, of W]
+        list_invs struct_invs upd VV''
+        VW unfolding eq
+      by blast
+    have confl_W: \<open>get_conflict_l W = None\<close> and
+      count_0_W: \<open>count_decided (get_trail_l W) = 0\<close>
+      by (use confl U''W'' VW'' VV'' count_0_V in
+        \<open>auto simp: eq twl_st_l_def cdcl_twl_restart.simps\<close>)[]
+       (use VW VV'' VW'' count_0_V in \<open>auto dest!: cdcl_twl_restart_l_count_dec simp: eq\<close>)
+
+    show ?thesis
+      unfolding eq[symmetric]
+      by (rule cdcl_GC_clauses_cdcl_twl_restart_l[OF VW'' list_invs struct_invs confl_W upd,
+           THEN order_trans])
+       (use count_0_W mark
+        cdcl_twl_restart_l_cdcl_twl_restart_l_is_cdcl_twl_restart_l[OF _ _ n_d, of U']
+       eq  in \<open>auto simp: \<open>V = V'\<close>\<close>)
+  qed
+    
+  have cdcl_twl_restart_l: \<open>cdcl_twl_restart_l_inp\<^sup>*\<^sup>* S X\<close>
+    if
+      \<open>T' \<in> Collect (?f1 S)\<close> and
+      \<open>U' \<in> Collect (?finp T')\<close> and
+      confl_U': \<open>\<not>get_conflict_l U' \<noteq> None\<close> and
+      V': \<open>V' \<in> Collect (?f2 U')\<close> and
+      \<open>W' \<in> Collect (?f3 V')\<close> and
+      \<open>X' \<in> Collect (?f3 W')\<close> and
+      \<open>(V, V') \<in> Id\<close> and
+      \<open>(T, T') \<in> Id\<close> and
+      \<open>(U, U') \<in> Id\<close> and
+      \<open>(W, W') \<in> Id\<close> and
+      \<open>(X,X') \<in> Id\<close>
+    for T T' U U' V V' W W' X X'
+    using that unfolding mem_Collect_eq
+    by (auto dest!: cdcl_twl_restart_l_inp.intros)
+
+  have abs_l_pre: \<open>restart_abs_l_pre S last_GC last_Restart False\<close>
+    using assms unfolding restart_abs_l_pre_def
+      restart_prog_pre_def apply -
+    apply (rule exI[of _ S'])
+    by auto
+
+  have simplify_clauses_with_unit_st:
+    \<open>simplify_clauses_with_unit_st T \<le> SPEC (?finp U)\<close>
+    if 
+      pre: \<open>cdcl_twl_full_restart_l_GC_prog_pre S\<close> and
+      \<open>(T, U) \<in> Id\<close> and
+      \<open>U \<in> Collect (?f1 S)\<close>
+   for T U
+ proof -
+   have st: \<open>T = U\<close> and
+     SU: \<open>S=U \<or> cdcl_twl_restart_l S U\<close> and
+     lev0: \<open>count_decided (get_trail_l U) = 0\<close>
+     using that by (auto dest!: cdcl_twl_restart_l_count_dec)
+
+   have confl: \<open>get_conflict_l U = None \<close>and
+     clss: \<open>clauses_to_update_l U = {#}\<close>
+     using pre SU upd
+     using confl SU upd by (auto simp add: cdcl_twl_full_restart_l_GC_prog_pre_def
+       cdcl_twl_restart_l.simps)
+
+   obtain V where
+     UV: \<open>(U, V) \<in> twl_st_l None\<close> and
+     struct: \<open>twl_struct_invs V\<close> and
+     list_invs: \<open>twl_list_invs U\<close> and
+     SUV: \<open>S = U \<or> cdcl_twl_restart S' V\<close>
+     using ST cdcl_twl_restart_l_invs[OF ST list_invs struct_invs] list_invs SU struct_invs
+       assms by blast
+
+   have ent: \<open>cdcl\<^sub>W_restart_mset.cdcl\<^sub>W_learned_clauses_entailed_by_init (state\<^sub>W_of S')\<close>
+      using assms(7) unfolding restart_prog_pre_def by blast
+   have 
+     ent: \<open>cdcl\<^sub>W_restart_mset.cdcl\<^sub>W_learned_clauses_entailed_by_init (state\<^sub>W_of V)\<close>
+     using cdcl_twl_restart_entailed_init[unfolded state\<^sub>W_of_def[symmetric], of S' V]
+       ent SUV UV ST by (auto simp: twl_st_l_def
+         cdcl\<^sub>W_restart_mset.cdcl\<^sub>W_learned_clauses_entailed_by_init_def)
+
+    show ?thesis
+      apply (rule simplify_clauses_with_unit_st_spec[THEN order_trans, of _ V])
+      apply (use lev0 UV struct list_invs st confl clss ent in auto)[7]
+      apply (auto dest: rtranclp_cdcl_twl_inprocessing_l_cdcl_twl_l_inp
+          rtranclp_cdcl_twl_inprocessing_l_count_dec simp: st lev0)
+      done
+  qed
+  show ?thesis
+    unfolding cdcl_twl_full_restart_inprocess_l_def
+    apply (rule order_trans)
+    prefer 2 apply (rule ref_two_step')
+    apply (rule alt_def)
+    apply refine_rcg
+    subgoal
+      using assms unfolding cdcl_twl_full_restart_l_GC_prog_pre_def restart_prog_pre_def
+      by fastforce
+    subgoal
+      by (rule cdcl_twl_local_restart_l_spec0_cdcl_twl_restart_l[THEN order_trans, OF abs_l_pre])
+        auto
+    subgoal for T U
+      by (rule simplify_clauses_with_unit_st)
+    subgoal by auto 
+    subgoal for T T' U U'
+      by (rule 1)
+    subgoal for T T' U U' V V'
       by (rule mark_to_delete_clauses_l_pre)
     subgoal for U U'
       by (rule 2)
@@ -666,14 +1157,47 @@ where
        RETURN (T, last_GC, size (get_all_learned_clss_l T), n)
      }
      else if b \<and> \<not>brk then do {
-       b \<leftarrow> SPEC(\<lambda>_. True);
-       T \<leftarrow> (if b then cdcl_twl_full_restart_l_prog S else cdcl_twl_full_restart_l_GC_prog S);
-       RETURN (T, size (get_all_learned_clss_l T), size (get_all_learned_clss_l T), n + 1)
+       inp \<leftarrow> inprocessing_required_l S;
+       if \<not>inp then do {
+         b \<leftarrow> SPEC(\<lambda>_. True);
+         T \<leftarrow> (if b then cdcl_twl_full_restart_l_prog S else cdcl_twl_full_restart_l_GC_prog S);
+         RETURN (T, size (get_all_learned_clss_l T), size (get_all_learned_clss_l T), n + 1)
+       }
+       else do {
+         T \<leftarrow> cdcl_twl_full_restart_inprocess_l S;
+         RETURN (T, size (get_all_learned_clss_l T), size (get_all_learned_clss_l T), n + 1)
+       }
      }
      else
        RETURN (S, last_GC, last_Restart, n)
    }\<close>
 
+lemma restart_prog_l_alt_def:
+     \<open>restart_prog_l S last_GC last_Restart n brk = do {
+     ASSERT(restart_abs_l_pre S last_GC last_Restart brk);
+     b \<leftarrow> GC_required_l S last_GC n;
+     b2 \<leftarrow> restart_required_l S last_Restart n;
+     if b2 \<and> \<not>brk then do {
+       T \<leftarrow> cdcl_twl_restart_l_prog S;
+       RETURN (T, last_GC, size (get_all_learned_clss_l T), n)
+     }
+     else if b \<and> \<not>brk then do {
+       inp \<leftarrow> inprocessing_required_l S;
+       if \<not>inp then do {
+         b \<leftarrow> SPEC(\<lambda>_. True);
+         T \<leftarrow> (if b then cdcl_twl_full_restart_l_prog S else cdcl_twl_full_restart_l_GC_prog S);
+         RETURN (T, size (get_all_learned_clss_l T), size (get_all_learned_clss_l T), n + 1)
+       }
+       else do {
+         T \<leftarrow> cdcl_twl_full_restart_inprocess_l S;
+         T \<leftarrow> RETURN T;
+         RETURN (T, size (get_all_learned_clss_l T), size (get_all_learned_clss_l T), n + 1)
+       }
+     }
+     else
+       RETURN (S, last_GC, last_Restart, n)
+   }\<close>
+   by (auto simp: restart_prog_l_def cong: if_cong)
 
 lemma restart_prog_l_restart_abs_l:
   \<open>(uncurry4 restart_prog_l, uncurry4 restart_abs_l)
@@ -711,8 +1235,7 @@ proof -
     \<open>cdcl_twl_full_restart_l_GC_prog S \<le> SPEC (cdcl_twl_restart_l S)\<close>
     if
       inv: \<open>restart_abs_l_pre S last_GC last_Restart brk\<close> and
-      brk: \<open>ba \<and> b2a \<and> \<not> brk\<close> and
-      lvl: \<open>count_decided (get_trail_l S) = 0\<close>
+      brk: \<open>ba \<and> b2a \<and> \<not> brk\<close>
     for ba b2a brk S last_GC last_Restart
   proof -
     obtain T where
@@ -729,7 +1252,7 @@ proof -
       by (auto simp: twl_st)
     show ?thesis
       by (rule cdcl_twl_full_restart_l_GC_prog_cdcl_twl_restart_l[unfolded Down_id_eq, OF ST list_invs
-        struct_invs confl upd stgy_invs inv2 lvl])
+        struct_invs confl upd stgy_invs inv2])
   qed
 
   have restart_abs_l_alt_def:
@@ -743,23 +1266,82 @@ proof -
      }
      else
      if b \<and> \<not>brk then do {
-       _ \<leftarrow> SPEC(\<lambda>b :: bool. True);
+       inp \<leftarrow> inprocessing_required_l S;
+     if \<not>inp then do {
+       _ \<leftarrow> SPEC(\<lambda>_::bool. True);
        T \<leftarrow> SPEC(\<lambda>T. cdcl_twl_restart_l S T);
        RETURN (T, size (get_all_learned_clss_l T), size (get_all_learned_clss_l T), n + 1)
+       }
+       else do {
+       T \<leftarrow> SPEC (\<lambda>T. cdcl_twl_restart_l_inp\<^sup>*\<^sup>* S T \<and> count_decided (get_trail_l T) = 0);
+       T \<leftarrow> SPEC(cdcl_twl_restart_l T);
+       RETURN (T, size (get_all_learned_clss_l T), size (get_all_learned_clss_l T), n + 1)
+       }
      }
      else
        RETURN (S, last_GC, last_Restart, n)
        }\<close> for  S last_GC last_Restart n brk
      unfolding restart_abs_l_def
      by (auto cong: if_cong)
+   have cdcl_twl_full_restart_inprocess_l:
+     \<open>cdcl_twl_full_restart_inprocess_l S \<le> SPEC (\<lambda>T. cdcl_twl_restart_l_inp\<^sup>*\<^sup>* S T \<and> count_decided (get_trail_l T) = 0)\<close>
+     if
+       inv: \<open>restart_abs_l_pre S last_GC last_Restart brk\<close> and
+       brk: \<open>ba \<and> b2a \<and> \<not> brk\<close>
+     for ba b2a brk S last_GC last_Restart
+   proof -
+     obtain T where
+       ST: \<open>(S, T) \<in> twl_st_l None\<close> and
+       struct_invs: \<open>twl_struct_invs T\<close> and
+       list_invs: \<open>twl_list_invs S\<close> and
+       upd: \<open>clauses_to_update_l S = {#}\<close> and
+       stgy_invs: \<open>twl_stgy_invs T\<close> and
+       confl: \<open>get_conflict_l S = None\<close> and
+       inv2: \<open>restart_prog_pre T last_GC last_Restart brk\<close> and
+       ent_init: \<open>cdcl\<^sub>W_restart_mset.cdcl\<^sub>W_learned_clauses_entailed_by_init (state\<^sub>W_of T)\<close>
+       using inv brk unfolding restart_abs_l_pre_def restart_prog_pre_def
+       apply - apply normalize_goal+
+       by (auto simp: twl_st)
+     show ?thesis
+       by (rule cdcl_twl_full_restart_inprocess_l_cdcl_twl_restart_l[THEN order_trans,
+         OF ST list_invs struct_invs confl upd stgy_invs inv2])
+         auto
+    qed
 
    have [simp]: \<open>cdcl_twl_restart_only_l S Ta \<Longrightarrow>clauses_to_update_l Ta = {#}\<close> for S Ta
      by (auto simp: cdcl_twl_restart_only_l.simps)
    have [simp]: \<open>cdcl_twl_restart_l S Ta \<Longrightarrow>clauses_to_update_l Ta = {#}\<close> for S Ta
      by (auto simp: cdcl_twl_restart_l.simps)
+   have \<open>(get_conflict_l T \<noteq> None) \<or> cdcl_twl_restart_l T' T\<close>
+     if 
+       \<open>restart_abs_l_pre S p m brk\<close> and
+       \<open>restart_abs_l_pre S p m brk\<close> and
+       \<open>(b, ba) \<in> bool_rel\<close> and
+       \<open>(b2, b2a) \<in> bool_rel\<close> and
+       \<open>\<not> (b2 \<and> \<not> brk)\<close> and
+       \<open>\<not> (b2a \<and> \<not> brk)\<close> and
+       \<open>b \<and> \<not> brk\<close> and
+       \<open>ba \<and> \<not> brk\<close> and
+       \<open>(inp, inp') \<in> bool_rel\<close> and
+       \<open>\<not> \<not> inp\<close> and
+       \<open>\<not> \<not> inp'\<close> and
+       TT': \<open>(T, T') \<in> Id\<close> and
+       T': \<open>T' \<in> {T. cdcl_twl_restart_l_inp\<^sup>*\<^sup>* S T \<and> count_decided (get_trail_l T) = 0}\<close>
+     for b ba b2 b2a inp inp' T T' S p m brk
+   proof -
+     have eq: \<open>T = T'\<close>
+       using TT' by auto
+         find_theorems "?a \<or> _" "\<not>?a"
+     show ?thesis
+       unfolding eq
+       apply (subst imp_conv_disj[symmetric], rule impI)
+       apply (rule cdcl_twl_restart_l_refl)
+         using T' apply auto
+       sorry
+   qed
    have \<open>restart_prog_l S p m n brk \<le> \<Down> (?R \<times>\<^sub>r nat_rel \<times>\<^sub>r nat_rel \<times>\<^sub>r nat_rel)
        (restart_abs_l S p m n brk)\<close> for S n brk p m
-    unfolding restart_prog_l_def restart_abs_l_alt_def restart_required_l_def cdcl_twl_restart_l_prog_def
+    unfolding restart_prog_l_alt_def restart_abs_l_alt_def restart_required_l_def cdcl_twl_restart_l_prog_def
     apply (refine_vcg)
     subgoal by auto
     subgoal
@@ -768,10 +1350,15 @@ proof -
     subgoal by (auto intro: cdcl_twl_restart_only_l_list_invs
       simp: restart_abs_l_pre_def)
     subgoal by auto
+    subgoal by auto
     subgoal by (rule cdcl_twl_full_restart_l_prog) auto
     subgoal by (rule cdcl_twl_full_restart_l_GC_prog) auto
     subgoal by (auto simp: cdcl_twl_restart_l_list_invs
       simp: restart_abs_l_pre_def)
+    subgoal by (rule cdcl_twl_full_restart_inprocess_l, assumption, auto)
+    subgoal for b ba b2 b2a inp inp' T T'
+      explore_have
+      sorry
     subgoal by (auto simp: cdcl_twl_restart_l_list_invs
       simp: restart_abs_l_pre_def)
     done
